Prove simulation of certification to pf step

src/prop/CapPFStep.v
@@ -17,93 +17,69 @@ Require Import Local.
 Require Import Thread.
 
 Require Import PromiseConsistent.
+Require Import PFStep.
 
 Set Implicit Arguments.
 
 Module CapPFStep.
-  Inductive sim_promises (promises_src promises_tgt: Memory.t): Prop :=
-  | sim_promises_intro
-      (SOUND: forall loc from to msg_src
-                (GET_SRC: Memory.get loc to promises_src = Some (from, msg_src)),
-          exists msg_tgt,
-            <<GET_TGT: Memory.get loc to promises_tgt = Some (from, msg_tgt)>>)
-      (COMPLETE: forall loc from to msg
-                   (GET_TGT: Memory.get loc to promises_tgt = Some (from, msg)),
-          <<GET_SRC: Memory.get loc to promises_src = Some (from, Message.half)>>)
-  .
+  Definition sim_promises := PFStep.sim_promises.
+  Hint Unfold sim_promises.
+  Definition sim_local := PFStep.sim_local.
+  Hint Unfold sim_local.
+  Definition sim_message := PFStep.sim_message.
 
-  Inductive sim_local (lc_src lc_tgt: Local.t): Prop :=
-  | sim_local_intro
-      (TVIEW: TView.le lc_src.(Local.tview) lc_tgt.(Local.tview))
-      (PROMISES: sim_promises lc_src.(Local.promises) lc_tgt.(Local.promises))
-  .
+  Definition cap_src (latests: TimeMap.t) (loc: Loc.t) (promises: Memory.t)
+             (msg_src: Message.t) (val: Const.t) (released_tgt: option View.t): Prop :=
+    if Memory.get loc (latests loc) promises
+    then msg_src = Message.half
+    else sim_message msg_src (Message.full val released_tgt).
 
-  Inductive sim_message: forall (msg_src msg_tgt: Message.t), Prop :=
-  | sim_message_full
-      val released_src released_tgt
-      (RELEASED: View.opt_le released_src released_tgt):
-      sim_message (Message.full val released_src) (Message.full val released_tgt)
-  | sim_message_half:
-      sim_message Message.half Message.half
-  .
-  Hint Constructors sim_message.
-
-  Program Instance sim_message_PreOrder: PreOrder sim_message.
-  Next Obligation.
-    ii. destruct x; econs; refl.
-  Qed.
-  Next Obligation.
-    ii. inv H; inv H0; econs. etrans; eauto.
-  Qed.
-
-  Inductive sim_memory (promises mem_src mem_tgt: Memory.t): Prop :=
+  Inductive sim_memory (latests caps: TimeMap.t) (promises mem_src mem_tgt: Memory.t): Prop :=
   | sim_memory_intro
       (SOUND: forall loc from to msg_src
+                (CAP: to <> caps loc)
                 (GETP: Memory.get loc to promises = None)
                 (GET_SRC: Memory.get loc to mem_src = Some (from, msg_src)),
           exists msg_tgt,
             <<GET_TGT: Memory.get loc to mem_tgt = Some (from, msg_tgt)>> /\
             <<MSG: sim_message msg_src msg_tgt>>)
       (COMPLETE: forall loc from to msg_tgt
+                   (CAP: to <> caps loc)
                    (GETP: Memory.get loc to promises = None)
                    (GET_TGT: Memory.get loc to mem_tgt = Some (from, msg_tgt)),
           exists msg_src,
             <<GET_SRC: Memory.get loc to mem_src = Some (from, msg_src)>> /\
             <<MSG: sim_message msg_src msg_tgt>>)
+      (LATESTS: forall loc, Time.lt (latests loc) (caps loc))
+      (CAPP: forall loc, Memory.get loc (caps loc) promises = None)
+      (CAPS: forall loc,
+          exists from_latest from val released msg_src released_tgt,
+            <<LATEST: Memory.get loc (latests loc) mem_tgt = Some (from_latest, Message.full val released)>> /\
+            <<CAP_SRC: Memory.get loc (caps loc) mem_src = Some (from, msg_src)>> /\
+            <<CAP_TGT: Memory.get loc (caps loc) mem_tgt = Some (from, Message.full val released_tgt)>> /\
+            <<MSG: cap_src latests loc promises msg_src val released_tgt>>)
   .
 
-  Inductive sim_thread (lang: Language.t) (e_src e_tgt: @Thread.t lang): Prop :=
+  Inductive sim_thread (lang: Language.t) (latests caps: TimeMap.t) (e_src e_tgt: @Thread.t lang): Prop :=
   | sim_thread_intro
       (STATE: e_src.(Thread.state) = e_tgt.(Thread.state))
       (LOCAL: sim_local e_src.(Thread.local) e_tgt.(Thread.local))
       (SC: TimeMap.le e_src.(Thread.sc) e_tgt.(Thread.sc))
-      (MEMORY: sim_memory e_tgt.(Thread.local).(Local.promises)
+      (MEMORY: sim_memory latests caps
+                          e_tgt.(Thread.local).(Local.promises)
                           e_src.(Thread.memory) e_tgt.(Thread.memory))
   .
 
 
-  Lemma sim_promises_get_src
-        promises_src promises_tgt
-        loc from to msg_src
-        (PROMISES: sim_promises promises_src promises_tgt)
-        (GET_SRC: Memory.get loc to promises_src = Some (from, msg_src)):
-    exists msg_tgt,
-      <<GET_TGT: Memory.get loc to promises_tgt = Some (from, msg_tgt)>> /\
-      <<MSG: msg_src = Message.half>>.
-  Proof.
-    inv PROMISES.
-    exploit SOUND; eauto. i. des.
-    exploit COMPLETE; eauto. i. des.
-    rewrite GET_SRC in x. inv x.
-    esplits; eauto.
-  Qed.
+  Definition sim_promises_get_src := PFStep.sim_promises_get_src.
 
   Lemma sim_memory_get_src
+        latests caps
         promises_src promises_tgt
         mem_src mem_tgt
         loc from to msg_src
         (PROMISES: sim_promises promises_src promises_tgt)
-        (MEM: sim_memory promises_tgt mem_src mem_tgt)
+        (MEM: sim_memory latests caps promises_tgt mem_src mem_tgt)
         (LE_SRC: Memory.le promises_src mem_src)
         (LE_TGT: Memory.le promises_tgt mem_tgt)
         (GET_SRC: Memory.get loc to mem_src = Some (from, msg_src)):
@@ -118,16 +94,22 @@ Module CapPFStep.
       exploit LE_SRC; eauto. i.
       rewrite GET_SRC in x1. inv x1.
       esplits; eauto. unguard. des; eauto.
-    - exploit SOUND0; eauto. i. des.
-      unguard. esplits; eauto.
+    - destruct (Time.eq_dec to (caps loc)).
+      + subst. specialize (CAPS loc). i. des.
+        rewrite GET_SRC in CAP_SRC. inv CAP_SRC.
+        esplits; eauto.
+        unguard. unfold cap_src in *. des_ifs; eauto.
+      + exploit SOUND0; eauto. i. des.
+        unguard. esplits; eauto.
   Qed.
 
   Lemma sim_memory_get_tgt
+        latests caps
         promises_src promises_tgt
         mem_src mem_tgt
         loc from to msg_tgt
         (PROMISES: sim_promises promises_src promises_tgt)
-        (MEM: sim_memory promises_tgt mem_src mem_tgt)
+        (MEM: sim_memory latests caps promises_tgt mem_src mem_tgt)
         (LE_SRC: Memory.le promises_src mem_src)
         (LE_TGT: Memory.le promises_tgt mem_tgt)
         (GET_TGT: Memory.get loc to mem_tgt = Some (from, msg_tgt)):
@@ -142,16 +124,22 @@ Module CapPFStep.
       exploit COMPLETE; eauto. i. des.
       exploit LE_SRC; eauto. i.
       esplits; eauto. unguard. des; eauto.
-    - exploit COMPLETE0; eauto. i. des.
-      unguard. esplits; eauto.
+    - destruct (Time.eq_dec to (caps loc)).
+      + subst. specialize (CAPS loc). des.
+        rewrite GET_TGT in CAP_TGT. inv CAP_TGT.
+        esplits; eauto.
+        unguard. unfold cap_src in *. des_ifs; eauto.
+      + exploit COMPLETE0; eauto. i. des.
+        unguard. esplits; eauto.
   Qed.
 
   Lemma promise
         msg_src
+        latests caps
         promises1_src mem1_src
         promises1_tgt mem1_tgt loc from to msg_tgt promises2_tgt mem2_tgt kind_tgt
         (PROMISES1: sim_promises promises1_src promises1_tgt)
-        (MEM1: sim_memory promises1_tgt mem1_src mem1_tgt)
+        (MEM1: sim_memory latests caps promises1_tgt mem1_src mem1_tgt)
         (LE1_SRC: Memory.le promises1_src mem1_src)
         (LE1_TGT: Memory.le promises1_tgt mem1_tgt)
         (CLOSED1_SRC: Memory.closed mem1_src)
@@ -163,7 +151,7 @@ Module CapPFStep.
       <<PROMISE_SRC: Memory.promise promises1_src mem1_src loc from to msg_src promises2_src mem2_src kind_src>> /\
       <<HALF: msg_src = Message.half ->
               <<PROMISES2: sim_promises promises2_src promises2_tgt>> /\
-              <<MEM2: sim_memory promises2_tgt mem2_src mem2_tgt>>>> /\
+              <<MEM2: sim_memory latests caps promises2_tgt mem2_src mem2_tgt>>>> /\
       <<KIND: Memory.op_kind_match kind_src kind_tgt>>.
   Proof.
     inv PROMISE_TGT.
@@ -202,6 +190,29 @@ Module CapPFStep.
           inv MEM1. eapply COMPLETE; eauto.
           destruct (Memory.get loc0 to0 promises1_tgt) as [[]|] eqn:GETP1; eauto.
           exploit Memory.add_get1; try exact GETP1; eauto. i. congr.
+      + apply MEM1.
+      + erewrite Memory.add_o; eauto. condtac; ss.
+        * des. subst.
+          exploit Memory.add_get0; try exact MEM. i. des.
+          inv MEM1. specialize (CAPS loc). des. congr.
+        * inv MEM1. specialize (CAPP loc0). ss.
+      + inv MEM1. clear SOUND COMPLETE.
+        exploit Memory.add_get0; try exact MEM. i. des.
+        erewrite Memory.add_o; eauto. condtac; ss.
+        * des. subst.
+          specialize (CAPS loc). des. congr.
+        * guardH o.
+          specialize (CAPS loc0). des.
+          destruct (loc_ts_eq_dec (loc, to) (loc0, (caps loc0))).
+          { ss. des. subst. congr. }
+          { ss. guardH o0. esplits; eauto.
+            - erewrite Memory.add_o; eauto. condtac; [|eauto].
+              ss. des. subst. congr.
+            - erewrite Memory.add_o; eauto. condtac; [|eauto].
+              ss. des. subst. congr.
+            - unfold cap_src in *. des_ifs; eauto.
+              + revert Heq. erewrite Memory.add_o; eauto. condtac; ss; congr.
+              + revert Heq. erewrite Memory.add_o; eauto. condtac; ss; congr. }
     - (* split *)
       exploit Memory.split_get0; try exact PROMISES. i. des.
       inv PROMISES1. exploit COMPLETE; try exact GET0. i. des.
@@ -246,6 +257,63 @@ Module CapPFStep.
           inv MEM1. eapply COMPLETE0; eauto.
           destruct (Memory.get loc0 to0 promises1_tgt) as [[]|] eqn:GETP1; eauto.
           exploit Memory.split_get1; try exact GETP1; eauto. i. des. congr.
+      + apply MEM1.
+      + erewrite Memory.split_o; eauto. repeat condtac; ss.
+        * des. subst.
+          exploit Memory.split_get0; try exact MEM. i. des.
+          inv MEM1. specialize (CAPS loc). des. congr.
+        * guardH o. des. subst.
+          exploit Memory.split_get0; try exact PROMISES. i. des.
+          inv MEM1. specialize (CAPP loc). congr.
+        * inv MEM1. specialize (CAPP loc0). ss.
+      + inv MEM1. clear SOUND COMPLETE SOUND0 COMPLETE0.
+        exploit Memory.split_get0; try exact MEM. i. des.
+        specialize (CAPS loc0). des.
+        erewrite Memory.split_o; eauto. repeat condtac; ss.
+        * des. subst. congr.
+        * des; subst; ss.
+          rewrite LATEST in GET4. inv GET4.
+          assert (TO: to <> caps loc).
+          { ii. subst. inv MEM. inv SPLIT.
+            specialize (LATESTS loc). rewrite LATESTS in TS23. timetac. }
+          esplits; eauto.
+          { erewrite Memory.split_o; eauto. repeat condtac; [| |eauto].
+            - ss. des. subst. congr.
+            - guardH o0. ss. des.
+              specialize (LATESTS loc). rewrite a0 in LATESTS. timetac. }
+          { erewrite Memory.split_o; eauto. repeat condtac; [| |eauto].
+            - ss. des. subst. congr.
+            - guardH o0. ss. des.
+              specialize (LATESTS loc). rewrite a0 in LATESTS. timetac. }
+          { unfold cap_src in *. des_ifs; eauto. }
+        * destruct (loc_ts_eq_dec (loc, to) (loc0, (caps loc0))); ss.
+          { des; subst; congr. }
+          destruct (loc_ts_eq_dec (loc, ts3) (loc0, (caps loc0))); ss.
+          { des; subst; ss. esplits; eauto.
+            - erewrite Memory.split_o; eauto. repeat condtac; [|eauto|].
+              + ss. des; subst; congr.
+              + ss. des; subst; congr.
+            - erewrite Memory.split_o; eauto. repeat condtac.
+              + ss. des; subst; congr.
+              + ss. rewrite CAP_TGT in GET4. inv GET4. ss.
+              + ss. des; subst; congr.
+            - unfold cap_src in *. des_ifs; eauto.
+              + revert Heq. erewrite Memory.split_o; eauto. repeat condtac; ss; congr.
+              + revert Heq. erewrite Memory.split_o; eauto. repeat condtac; ss.
+                guardH o2. guardH o3.
+                exploit Memory.split_get0; try exact x2. i. des.
+                rewrite CAP_SRC in GET8. inv GET8. inv MSG. }
+          { guardH o. guardH o0. guardH o1. guardH o2.
+            esplits; eauto.
+            - erewrite Memory.split_o; eauto. repeat condtac; [| |eauto]; ss.
+              + des. subst. congr.
+              + unguard. des; subst; congr.
+            - erewrite Memory.split_o; eauto. repeat condtac; [| |eauto]; ss.
+              + des. subst. congr.
+              + unguard. des; subst; congr.
+            - unfold cap_src in *. des_ifs; eauto.
+              + revert Heq. erewrite Memory.split_o; eauto. repeat condtac; ss; congr.
+              + revert Heq. erewrite Memory.split_o; eauto. repeat condtac; ss; congr. }
     - (* lower *)
       exploit Memory.lower_get0; try exact PROMISES. i. des.
       inv PROMISES1. exploit COMPLETE; eauto. i. des.
@@ -281,13 +349,57 @@ Module CapPFStep.
           inv MEM1. eapply COMPLETE0; eauto.
           destruct (Memory.get loc0 to0 promises1_tgt) as [[]|] eqn:GETP1; eauto.
           exploit Memory.lower_get1; try exact GETP1; eauto. i. des. congr.
+      + apply MEM1.
+      + erewrite Memory.lower_o; eauto. condtac; ss.
+        * des. subst.
+          exploit Memory.lower_get0; try exact PROMISES. i. des.
+          inv MEM1. specialize (CAPP loc). congr.
+        * inv MEM1. specialize (CAPP loc0). ss.
+      + inv MEM1. clear SOUND COMPLETE SOUND0 COMPLETE0.
+        exploit Memory.lower_get0; try exact MEM. i. des.
+        specialize (CAPS loc0). des.
+        erewrite Memory.lower_o; eauto. condtac; ss.
+        * des. subst.
+          rewrite LATEST in GET1. inv GET1. inv MSG_LE0.
+          esplits; eauto.
+          { erewrite Memory.lower_o; eauto. condtac; [|eauto].
+            ss. des. specialize (LATESTS loc).
+            rewrite a0 in *. timetac. }
+          { erewrite Memory.lower_o; eauto. condtac; [|eauto].
+            ss. des. specialize (LATESTS loc).
+            rewrite a0 in *. timetac. }
+          { unfold cap_src in *. des_ifs; eauto. }
+        * guardH o.
+          destruct (loc_ts_eq_dec (loc, to) (loc0, (caps loc0))).
+          { ss. des. subst.
+            rewrite CAP_TGT in GET1. inv GET1. inv MSG_LE0.
+            esplits; eauto.
+            - erewrite Memory.lower_o; eauto. condtac; [eauto|].
+              ss. des; congr.
+            - unfold cap_src in *. des_ifs; eauto.
+              + destruct p.
+                exploit Memory.lower_get1; try exact Heq0; eauto. i. des. congr.
+              + exploit Memory.lower_get1; try exact CAP_SRC; eauto. i. des.
+                exploit Memory.lower_get0; try exact x2. i. des.
+                inv MSG. inv MSG_LE0. congr. }
+          { ss. guardH o0.
+            esplits; eauto.
+            - erewrite Memory.lower_o; eauto. condtac;[|eauto].
+              ss. unguard. des; subst; ss.
+            - erewrite Memory.lower_o; eauto. condtac;[|eauto].
+              ss. unguard. des; subst; ss.
+            - unfold cap_src in *. des_ifs; eauto.
+              + revert Heq. erewrite Memory.lower_o; eauto. condtac; ss. congr.
+              + destruct p.
+                exploit Memory.lower_get1; try exact Heq0; eauto. i. des. congr. }
   Qed.
 
   Lemma promise_step
+        latests caps
         lc1_src mem1_src
         lc1_tgt mem1_tgt loc from to msg lc2_tgt mem2_tgt kind_tgt
         (LOCAL1: sim_local lc1_src lc1_tgt)
-        (MEM1: sim_memory lc1_tgt.(Local.promises) mem1_src mem1_tgt)
+        (MEM1: sim_memory latests caps lc1_tgt.(Local.promises) mem1_src mem1_tgt)
         (WF1_SRC: Local.wf lc1_src mem1_src)
         (WF1_TGT: Local.wf lc1_tgt mem1_tgt)
         (CLOSED1_SRC: Memory.closed mem1_src)
@@ -296,7 +408,7 @@ Module CapPFStep.
     exists lc2_src mem2_src kind_src,
       <<STEP_SRC: Local.promise_step lc1_src mem1_src loc from to Message.half lc2_src mem2_src kind_src>> /\
       <<LOCAL2: sim_local lc2_src lc2_tgt>> /\
-      <<MEM2: sim_memory lc2_tgt.(Local.promises) mem2_src mem2_tgt>>.
+      <<MEM2: sim_memory latests caps lc2_tgt.(Local.promises) mem2_src mem2_tgt>>.
   Proof.
     inv STEP_TGT.
     exploit promise; try exact PROMISE; eauto.
@@ -309,20 +421,25 @@ Module CapPFStep.
     esplits; eauto. econs; eauto. apply LOCAL1.
   Qed.
 
-  Lemma read_promise_None
-        lc1 mem1 loc to val released ord lc2
-        (WF1: Local.wf lc1 mem1)
-        (STEP: Local.read_step lc1 mem1 loc to val released ord lc2)
+  Definition read_promise_None := PFStep.read_promise_None.
+
+  Lemma read_cap
+        latests caps mem1_src
+        lc1 mem1_tgt loc val released ord lc2
+        (MEM1: sim_memory latests caps lc1.(Local.promises) mem1_src mem1_tgt)
+        (WF1: Local.wf lc1 mem1_tgt)
+        (STEP: Local.read_step lc1 mem1_tgt loc (caps loc) val released ord lc2)
         (CONS: promise_consistent lc2):
-    Memory.get loc to lc1.(Local.promises) = None.
+    Memory.get loc (latests loc) lc1.(Local.promises) = None.
   Proof.
-    destruct (Memory.get loc to lc1.(Local.promises)) as [[from msg]|] eqn:GETP; ss.
+    destruct (Memory.get loc (latests loc) (Local.promises lc1)) as [[]|] eqn:PROMISE; ss.
     exfalso.
-    inv WF1. inv STEP. exploit PROMISES; eauto. i.
-    rewrite GET in x. inv x.
-    exploit CONS; eauto. ss. i.
+    inv STEP. exploit CONS; eauto. i.
     eapply Time.lt_strorder.
-    eapply TimeFacts.le_lt_lt; eauto.
+    etrans; eauto.
+    inv MEM1. clear SOUND COMPLETE CAPS.
+    specialize (LATESTS loc).
+    eapply TimeFacts.lt_le_lt; eauto. ss.
     etrans; [|apply Time.join_l]. etrans; [|apply Time.join_r].
     unfold View.singleton_ur_if. condtac; ss.
     - unfold TimeMap.singleton.
@@ -334,10 +451,11 @@ Module CapPFStep.
   Qed.
 
   Lemma read_step
+        latests caps
         lc1_src mem1_src
         lc1_tgt mem1_tgt loc to val released_tgt ord lc2_tgt
         (LOCAL1: sim_local lc1_src lc1_tgt)
-        (MEM1: sim_memory lc1_tgt.(Local.promises) mem1_src mem1_tgt)
+        (MEM1: sim_memory latests caps lc1_tgt.(Local.promises) mem1_src mem1_tgt)
         (WF1_SRC: Local.wf lc1_src mem1_src)
         (WF1_TGT: Local.wf lc1_tgt mem1_tgt)
         (CLOSED1_SRC: Memory.closed mem1_src)
@@ -350,30 +468,51 @@ Module CapPFStep.
       <<RELEASED: View.opt_le released_src released_tgt>>.
   Proof.
     exploit read_promise_None; try exact STEP_TGT; eauto. i.
-    inv MEM1. inv LOCAL1. inv STEP_TGT.
-    exploit COMPLETE; eauto. i. des. inv MSG.
-    esplits.
-    - econs; eauto.
-      inv READABLE. inv TVIEW. econs; eauto.
-      + etrans; try exact PLN. apply CUR.
-      + i. exploit RLX; eauto. i.
-        etrans; try exact x. apply CUR.
-    - econs; eauto. ss.
-      eapply TViewFacts.read_tview_mon; eauto.
-      { apply WF1_TGT. }
-      { inv CLOSED1_TGT. exploit CLOSED; eauto. i. des.
-        inv MSG_WF. ss. }
-      { refl. }
-    - auto.
+    destruct (Time.eq_dec to (caps loc)).
+    - subst. exploit read_cap; eauto. i.
+      inv MEM1. clear SOUND COMPLETE LATESTS.
+      specialize (CAPS loc). des.
+      unfold cap_src in *. rewrite x1 in *. inv MSG.
+      inv LOCAL1.
+      inv STEP_TGT. rewrite CAP_TGT in GET. inv GET.
+      esplits.
+      + econs; eauto.
+        inv READABLE. inv TVIEW. econs; eauto.
+        * etrans; try exact PLN. apply CUR.
+        * i. exploit RLX; eauto. i.
+          etrans; try exact x. apply CUR.
+      + econs; eauto. ss.
+        eapply TViewFacts.read_tview_mon; eauto.
+        { apply WF1_TGT. }
+        { inv CLOSED1_TGT. exploit CLOSED; eauto. i. des.
+          inv MSG_WF. ss. }
+        { refl. }
+      + auto.
+    - inv MEM1. inv LOCAL1. inv STEP_TGT.
+      exploit COMPLETE; eauto. i. des. inv MSG.
+      esplits.
+      + econs; eauto.
+        inv READABLE. inv TVIEW. econs; eauto.
+        * etrans; try exact PLN. apply CUR.
+        * i. exploit RLX; eauto. i.
+          etrans; try exact x. apply CUR.
+      + econs; eauto. ss.
+        eapply TViewFacts.read_tview_mon; eauto.
+        { apply WF1_TGT. }
+        { inv CLOSED1_TGT. exploit CLOSED; eauto. i. des.
+          inv MSG_WF. ss. }
+        { refl. }
+      + auto.
   Qed.
 
   Lemma promise_remove_sim
+        latests caps
         promises1_src mem1_src loc from to msg_src promises2_src mem2_src kind_src
         promises3_src
         promises1_tgt mem1_tgt msg_tgt promises2_tgt mem2_tgt kind_tgt
         promises3_tgt
         (PROMISES1: sim_promises promises1_src promises1_tgt)
-        (MEM1: sim_memory promises1_tgt mem1_src mem1_tgt)
+        (MEM1: sim_memory latests caps promises1_tgt mem1_src mem1_tgt)
         (LE1_SRC: Memory.le promises1_src mem1_src)
         (LE1_TGT: Memory.le promises1_tgt mem1_tgt)
         (CLOSED1_SRC: Memory.closed mem1_src)
@@ -383,9 +522,10 @@ Module CapPFStep.
         (PROMISE_SRC: Memory.promise promises1_src mem1_src loc from to msg_src promises2_src mem2_src kind_src)
         (REMOVE_SRC: Memory.remove promises2_src loc from to msg_src promises3_src)
         (PROMISE_TGT: Memory.promise promises1_tgt mem1_tgt loc from to msg_tgt promises2_tgt mem2_tgt kind_tgt)
-        (REMOVE_TGT: Memory.remove promises2_tgt loc from to msg_tgt promises3_tgt):
-      <<PROMISES2: sim_promises promises3_src promises3_tgt>> /\
-      <<MEM2: sim_memory promises3_tgt mem2_src mem2_tgt>>.
+        (REMOVE_TGT: Memory.remove promises2_tgt loc from to msg_tgt promises3_tgt)
+        (TO: to <> latests loc):
+    <<PROMISES2: sim_promises promises3_src promises3_tgt>> /\
+    <<MEM2: sim_memory latests caps promises3_tgt mem2_src mem2_tgt>>.
   Proof.
     split; econs; i.
     - erewrite Memory.remove_o; eauto. condtac; ss.
@@ -475,24 +615,233 @@ Module CapPFStep.
           revert GET_TGT. erewrite Memory.lower_o; eauto. condtac; ss. i.
           revert GETP. erewrite Memory.lower_o; eauto. condtac; ss. i.
           inv MEM1. eauto.
+    - apply MEM1.
+    - erewrite Memory.remove_o; eauto. condtac; ss.
+      guardH o. inv PROMISE_SRC; inv PROMISE_TGT; inv KIND.
+      + erewrite Memory.add_o; eauto. condtac; ss.
+        inv MEM1. eauto.
+      + erewrite Memory.split_o; eauto. repeat condtac; ss.
+        * guardH o0. des. subst.
+          exploit Memory.split_get0; try exact PROMISES0. i. des.
+          inv MEM1. specialize (CAPP loc). congr.
+        * inv MEM1. eauto.
+      + erewrite Memory.lower_o; eauto. condtac; ss.
+        inv MEM1. eauto.
+    - inv MEM1. clear SOUND COMPLETE.
+      specialize (CAPS loc0). des.
+      inv PROMISE_SRC; inv PROMISE_TGT; inv KIND.
+      + erewrite Memory.add_o; eauto. condtac; ss.
+        * des. subst. congr.
+        * guardH o. esplits; eauto.
+          { erewrite Memory.add_o; eauto. condtac; [|eauto].
+            ss. des. subst.
+            exploit Memory.add_get0; try exact MEM. i. des. congr. }
+          { erewrite Memory.add_o; eauto. condtac; [|eauto].
+            ss. des. subst.
+            exploit Memory.add_get0; try exact MEM. i. des. congr. }
+          { unfold cap_src in *. des_ifs; eauto.
+            - revert Heq. erewrite Memory.remove_o; eauto. condtac; ss.
+              erewrite Memory.add_o; eauto. condtac; ss. congr.
+            - revert Heq. erewrite Memory.remove_o; eauto. condtac; ss.
+              erewrite Memory.add_o; eauto. condtac; ss. congr. }
+      + erewrite Memory.split_o; eauto. repeat condtac; ss.
+        * des. subst. congr.
+        * guardH o. des. subst.
+          exploit Memory.split_get0; try exact MEM0. i. des.
+          rewrite LATEST in *. inv GET0.
+          esplits; eauto.
+          { erewrite Memory.split_o; eauto. repeat condtac; [| |eauto]; ss.
+            - des. subst.
+              inv MEM0. inv SPLIT. specialize (LATESTS loc).
+              rewrite LATESTS in TS23. timetac.
+            - guardH o0. des. subst.
+              specialize (LATESTS loc). rewrite a0 in *. timetac. }
+          { erewrite Memory.split_o; eauto. repeat condtac; [| |eauto]; ss.
+            - des. subst.
+              inv MEM0. inv SPLIT. specialize (LATESTS loc).
+              rewrite LATESTS in TS23. timetac.
+            - guardH o0. des. subst.
+              specialize (LATESTS loc). rewrite a0 in *. timetac. }
+          { unfold cap_src in *. des_ifs; eauto.
+            - revert Heq. erewrite Memory.remove_o; eauto. condtac; ss.
+              erewrite Memory.split_o; eauto. repeat condtac; ss.
+              exploit Memory.split_get0; try exact PROMISES0. i. des; congr.
+            - revert Heq. erewrite Memory.remove_o; eauto. condtac; ss.
+              erewrite Memory.split_o; eauto. repeat condtac; ss. }
+        * guardH o. guardH o0.
+          exploit Memory.split_get0; try exact MEM0. i. des.
+          esplits; eauto.
+          { erewrite Memory.split_o; eauto. repeat condtac; [| |eauto]; ss.
+            - des. subst.
+              exploit Memory.split_get0; try exact MEM0. i. des. congr.
+            - guardH o1. des. subst.
+              exploit Memory.split_get0; try exact PROMISES0. i. des. congr. }
+          { erewrite Memory.split_o; eauto. repeat condtac; [| |eauto]; ss.
+            - des. subst.
+              exploit Memory.split_get0; try exact MEM0. i. des. congr.
+            - guardH o1. des. subst.
+              exploit Memory.split_get0; try exact PROMISES0. i. des. congr. }
+          { unfold cap_src in *. des_ifs; eauto.
+            - revert Heq. erewrite Memory.remove_o; eauto. condtac; ss.
+              erewrite Memory.split_o; eauto. repeat condtac; ss.
+              exploit Memory.split_get0; try exact PROMISES0. i. des; congr.
+            - revert Heq. erewrite Memory.remove_o; eauto. condtac; ss.
+              erewrite Memory.split_o; eauto. repeat condtac; ss. congr. }
+      + erewrite Memory.lower_o; eauto. condtac; ss.
+        * des. subst. congr.
+        * guardH o. esplits; eauto.
+          { erewrite Memory.lower_o; eauto. condtac; [|eauto].
+            ss. des. subst.
+            exploit Memory.lower_get0; try exact PROMISES0. i. des.
+            rewrite CAPP in *. congr. }
+          { erewrite Memory.lower_o; eauto. condtac; [|eauto].
+            ss. des. subst.
+            exploit Memory.lower_get0; try exact PROMISES0. i. des.
+            rewrite CAPP in *. congr. }
+          { unfold cap_src in *. des_ifs; eauto.
+            - revert Heq. erewrite Memory.remove_o; eauto. condtac; ss.
+              erewrite Memory.lower_o; eauto. condtac; ss. congr.
+            - revert Heq. erewrite Memory.remove_o; eauto. condtac; ss.
+              erewrite Memory.lower_o; eauto. condtac; ss. congr. }
   Qed.
 
-  Lemma view_opt_le_time_le
-        v1 v2 loc
-        (LE: View.opt_le v1 v2):
-    Time.le (v1.(View.unwrap).(View.rlx) loc) (v2.(View.unwrap).(View.rlx) loc).
+  Lemma promise_remove_sim_cap
+        latests caps
+        promises1_src mem1_src loc from msg_src promises2_src mem2_src kind_src
+        promises3_src
+        promises1_tgt mem1_tgt msg_tgt promises2_tgt mem2_tgt kind_tgt
+        promises3_tgt
+        (PROMISES1: sim_promises promises1_src promises1_tgt)
+        (MEM1: sim_memory latests caps promises1_tgt mem1_src mem1_tgt)
+        (LE1_SRC: Memory.le promises1_src mem1_src)
+        (LE1_TGT: Memory.le promises1_tgt mem1_tgt)
+        (CLOSED1_SRC: Memory.closed mem1_src)
+        (CLOSED1_TGT: Memory.closed mem1_tgt)
+        (MSG: sim_message msg_src msg_tgt)
+        (KIND: Memory.op_kind_match kind_src kind_tgt)
+        (PROMISE_SRC: Memory.promise promises1_src mem1_src loc from (latests loc) msg_src promises2_src mem2_src kind_src)
+        (REMOVE_SRC: Memory.remove promises2_src loc from (latests loc) msg_src promises3_src)
+        (PROMISE_TGT: Memory.promise promises1_tgt mem1_tgt loc from (latests loc) msg_tgt promises2_tgt mem2_tgt kind_tgt)
+        (REMOVE_TGT: Memory.remove promises2_tgt loc from (latests loc) msg_tgt promises3_tgt):
+    exists from_cap val mem3_src,
+      <<MSG: sim_message (Message.full val None) msg_tgt>> /\
+      <<LOWER: Memory.lower mem2_src loc from_cap (caps loc) Message.half (Message.full val None) mem3_src>> /\
+      <<PROMISES2: sim_promises promises3_src promises3_tgt>> /\
+      <<MEM2: sim_memory latests caps promises3_tgt mem3_src mem2_tgt>>.
   Proof.
-    inv LE; ss.
-    - unfold TimeMap.bot. apply Time.bot_spec.
-    - inv LE0. ss.
+    inv PROMISE_SRC; inv PROMISE_TGT; inv KIND.
+    { inv MEM1. specialize (CAPS loc). des.
+      exploit Memory.add_get0; try exact MEM0. i. des. congr. }
+    { inv MEM1. specialize (CAPS loc). des.
+      exploit Memory.split_get0; try exact MEM0. i. des. congr. }
+    dup MEM1. inv MEM2. clear SOUND COMPLETE LATESTS CAPP.
+    specialize (CAPS loc). des.
+    exploit Memory.lower_get0; try exact MEM0. i. des.
+    rewrite LATEST in *. inv GET. inv MSG_LE. inv MSG. clear GET0.
+    exploit Memory.lower_get0; try exact PROMISES0. i. des.
+    unfold cap_src in *. rewrite GET in *. subst.
+    clear GET GET0 MSG_LE.
+    exploit (@Memory.lower_exists mem2_src loc from0 (caps loc) Message.half (Message.full val None)).
+    { erewrite Memory.lower_o; eauto. condtac; ss. des.
+      inv MEM1. specialize (LATESTS loc).
+      rewrite a0 in *. timetac. }
+    { exploit Memory.get_ts; try exact CAP_SRC. i. des; ss.
+      inv MEM1. specialize (LATESTS loc).
+      rewrite x1 in *. inv LATESTS. }
+    { econs. ss. }
+    { econs. }
+    i. des.
+    rename x0 into LOWER. rename mem2 into mem3_src.
+    esplits; eauto; econs; ss; i.
+    - erewrite Memory.remove_o; eauto. condtac; ss.
+      + des. subst.
+        revert GET_SRC. erewrite Memory.remove_o; eauto. condtac; ss.
+      + revert GET_SRC. erewrite Memory.remove_o; eauto. condtac; ss. i.
+        guardH o. guardH o0.
+        erewrite Memory.lower_o; eauto. condtac; ss.
+        revert GET_SRC. erewrite Memory.lower_o; eauto. condtac; ss. i.
+        inv PROMISES1. eauto.
+    - erewrite Memory.remove_o; eauto. condtac; ss.
+      + des. subst.
+        revert GET_TGT. erewrite Memory.remove_o; eauto. condtac; ss.
+      + revert GET_TGT. erewrite Memory.remove_o; eauto. condtac; ss. i.
+        guardH o. guardH o0.
+        erewrite Memory.lower_o; eauto. condtac; ss.
+        revert GET_TGT. erewrite Memory.lower_o; eauto. condtac; ss. i.
+        inv PROMISES1. eauto.
+    - revert GETP. erewrite Memory.remove_o; eauto. condtac; ss; i.
+      + des. subst.
+        revert GET_SRC.
+        erewrite Memory.lower_o; eauto. condtac; des; ss.
+        erewrite Memory.lower_o; eauto. condtac; des; ss. i. inv GET_SRC.
+        erewrite Memory.lower_o; eauto. condtac; des; ss.
+        esplits; eauto. econs. ss.
+      + guardH o.
+        erewrite Memory.lower_o; eauto. condtac; ss.
+        revert GET_SRC. erewrite Memory.lower_o; eauto. condtac; ss.
+        { guardH o0. des. subst. ss. }
+        erewrite Memory.lower_o; eauto. condtac; ss; i.
+        revert GETP. erewrite Memory.lower_o; eauto. condtac; ss. i.
+        inv MEM1. eauto.
+    - revert GETP. erewrite Memory.remove_o; eauto. condtac; ss; i.
+      + des. subst.
+        revert GET_TGT.
+        erewrite Memory.lower_o; eauto. condtac; des; ss. i. inv GET_TGT.
+        erewrite Memory.lower_o; eauto. condtac; des; ss. i.
+        erewrite Memory.lower_o; eauto. condtac; des; ss.
+        esplits; eauto. econs. ss.
+      + guardH o.
+        erewrite Memory.lower_o; eauto. condtac; ss.
+        { des. subst. ss. }
+        erewrite Memory.lower_o; eauto. condtac; ss.
+        revert GET_TGT. erewrite Memory.lower_o; eauto. condtac; ss. i.
+        revert GETP. erewrite Memory.lower_o; eauto. condtac; ss. i.
+        inv MEM1. eauto.
+    - apply MEM1.
+    - erewrite Memory.remove_o; eauto. condtac; ss.
+      erewrite Memory.lower_o; eauto. condtac; ss.
+      inv MEM1. eauto.
+    - erewrite Memory.lower_o; eauto. condtac; ss.
+      + inv MEM1. clear SOUND COMPLETE CAPS.
+        des. subst. specialize (LATESTS loc).
+        exploit Memory.lower_get0; try exact LOWER. i. des.
+        esplits; eauto.
+        * erewrite Memory.lower_o; eauto. condtac; [|eauto].
+          ss. des. rewrite a1 in *. timetac.
+        * unfold cap_src in *. des_ifs; eauto.
+          { revert Heq. erewrite Memory.remove_o; eauto. condtac; ss. }
+          { econs. ss. }
+      + destruct (Loc.eq_dec loc0 loc).
+        { subst. des; ss. }
+        clear o COND.
+        inv MEM1. clear SOUND COMPLETE.
+        specialize (CAPS loc0). des.
+        esplits; eauto.
+        * erewrite Memory.lower_o; eauto. condtac.
+          { simpl in a. des. congr. }
+          erewrite Memory.lower_o; eauto. condtac; [|eauto].
+          ss. guardH o. des. ss.
+        * erewrite Memory.lower_o; eauto. condtac; [|eauto].
+          ss. des. congr.
+        * unfold cap_src in *. des_ifs; eauto.
+          { revert Heq.
+            erewrite Memory.remove_o; eauto. condtac; ss.
+            erewrite Memory.lower_o; eauto. condtac; ss. congr. }
+          { revert Heq.
+            erewrite Memory.remove_o; eauto. condtac; ss.
+            - des. subst. congr.
+            - erewrite Memory.lower_o; eauto. condtac; ss. congr. }
   Qed.
+
+  Definition view_opt_le_time_le := PFStep.view_opt_le_time_le.
 
   Lemma write_step
+        latests caps
         lc1_src sc1_src mem1_src releasedm_src
         lc1_tgt sc1_tgt mem1_tgt loc from to val releasedm_tgt released_tgt ord lc2_tgt sc2_tgt mem2_tgt kind_tgt
         (LOCAL1: sim_local lc1_src lc1_tgt)
         (SC1: TimeMap.le sc1_src sc1_tgt)
-        (MEM1: sim_memory lc1_tgt.(Local.promises) mem1_src mem1_tgt)
+        (MEM1: sim_memory latests caps lc1_tgt.(Local.promises) mem1_src mem1_tgt)
         (WF1_SRC: Local.wf lc1_src mem1_src)
         (WF1_TGT: Local.wf lc1_tgt mem1_tgt)
         (SC1_SRC: Memory.closed_timemap sc1_src mem1_src)
@@ -503,13 +852,14 @@ Module CapPFStep.
         (RELEASEDM_TGT: View.opt_wf releasedm_tgt)
         (RELEASEDM: View.opt_le releasedm_src releasedm_tgt)
         (STEP_TGT: Local.write_step lc1_tgt sc1_tgt mem1_tgt loc from to val
-                                    releasedm_tgt released_tgt ord lc2_tgt sc2_tgt mem2_tgt kind_tgt):
+                                    releasedm_tgt released_tgt ord lc2_tgt sc2_tgt mem2_tgt kind_tgt)
+        (TO: to <> latests loc):
     exists released_src lc2_src sc2_src mem2_src kind_src,
       <<STEP_SRC: Local.write_step lc1_src sc1_src mem1_src loc from to val
                                    releasedm_src released_src ord lc2_src sc2_src mem2_src kind_src>> /\
       <<LOCAL2: sim_local lc2_src lc2_tgt>> /\
       <<SC2: TimeMap.le sc2_src sc2_tgt>> /\
-      <<MEM2: sim_memory lc2_tgt.(Local.promises) mem2_src mem2_tgt>>.
+      <<MEM2: sim_memory latests caps lc2_tgt.(Local.promises) mem2_src mem2_tgt>>.
   Proof.
     inv STEP_TGT. inv WRITE.
     exploit (@promise (Message.full val (TView.write_released lc1_src.(Local.tview) sc1_src loc to releasedm_src ord)));
@@ -546,39 +896,137 @@ Module CapPFStep.
     - ss.
   Qed.
 
-  Lemma fence_step
-        lc1_src sc1_src mem1_src
-        lc1_tgt sc1_tgt mem1_tgt ordr ordw lc2_tgt sc2_tgt
+  Lemma write_step_cap
+        latests caps
+        lc1_src sc1_src mem1_src releasedm_src
+        lc1_tgt sc1_tgt mem1_tgt loc from val releasedm_tgt released_tgt ord lc2_tgt sc2_tgt mem2_tgt kind_tgt
         (LOCAL1: sim_local lc1_src lc1_tgt)
         (SC1: TimeMap.le sc1_src sc1_tgt)
+        (MEM1: sim_memory latests caps lc1_tgt.(Local.promises) mem1_src mem1_tgt)
         (WF1_SRC: Local.wf lc1_src mem1_src)
         (WF1_TGT: Local.wf lc1_tgt mem1_tgt)
-        (STEP_TGT: Local.fence_step lc1_tgt sc1_tgt ordr ordw lc2_tgt sc2_tgt):
-    exists lc2_src sc2_src,
-      <<STEP_SRC: Local.fence_step lc1_src sc1_src ordr ordw lc2_src sc2_src>> /\
+        (SC1_SRC: Memory.closed_timemap sc1_src mem1_src)
+        (SC1_TGT: Memory.closed_timemap sc1_tgt mem1_tgt)
+        (CLOSED1_SRC: Memory.closed mem1_src)
+        (CLOSED1_TGT: Memory.closed mem1_tgt)
+        (RELEASEDM_SRC: View.opt_wf releasedm_src)
+        (RELEASEDM_TGT: View.opt_wf releasedm_tgt)
+        (RELEASEDM: View.opt_le releasedm_src releasedm_tgt)
+        (STEP_TGT: Local.write_step lc1_tgt sc1_tgt mem1_tgt loc from (latests loc) val
+                                    releasedm_tgt released_tgt ord lc2_tgt sc2_tgt mem2_tgt kind_tgt):
+    exists released_src lc2_src sc2_src mem2_src kind_src from_cap mem3_src,
+      <<STEP_SRC: Local.write_step lc1_src sc1_src mem1_src loc from (latests loc) val
+                                   releasedm_src released_src ord lc2_src sc2_src mem2_src kind_src>> /\
+      <<LOWER: Memory.lower mem2_src loc from_cap (caps loc) Message.half (Message.full val None) mem3_src>> /\
       <<LOCAL2: sim_local lc2_src lc2_tgt>> /\
-      <<SC2: TimeMap.le sc2_src sc2_tgt>>.
+      <<SC2: TimeMap.le sc2_src sc2_tgt>> /\
+      <<MEM2: sim_memory latests caps lc2_tgt.(Local.promises) mem3_src mem2_tgt>>.
   Proof.
-    esplits.
-    - econs; eauto. ii. inv LOCAL1.
-      exploit sim_promises_get_src; eauto. i. des. subst. ss.
-    - inv STEP_TGT. inv LOCAL1. econs; eauto. ss.
-      eapply TViewFacts.write_fence_tview_mon; try refl; ss.
-      + eapply TViewFacts.read_fence_tview_mon; try refl; ss.
-        apply WF1_TGT.
-      + eapply TViewFacts.read_fence_future; apply WF1_SRC.
-    - inv STEP_TGT. inv LOCAL1.
-      eapply TViewFacts.write_fence_sc_mon; try refl; ss.
-      eapply TViewFacts.read_fence_tview_mon; try refl; ss.
-      apply WF1_TGT.
+    inv STEP_TGT. inv WRITE.
+    exploit (@promise (Message.full val (TView.write_released lc1_src.(Local.tview) sc1_src loc (latests loc) releasedm_src ord)));
+      try exact PROMISE; eauto.
+    { apply LOCAL1. }
+    { apply WF1_SRC. }
+    { apply WF1_TGT. }
+    { econs. eapply TViewFacts.write_future0; ss. apply WF1_SRC. }
+    { econs. etrans; try by (inv PROMISE; inv TS; eauto).
+      apply view_opt_le_time_le.
+      apply TViewFacts.write_released_mon; try refl; ss.
+      - apply LOCAL1.
+      - apply WF1_TGT. }
+    i. des.
+    exploit Memory.promise_get0; try exact PROMISE_SRC. i. des.
+    exploit Memory.remove_exists; try exact GET_PROMISES. i. des.
+    exploit promise_remove_sim_cap; try eapply LOCAL1; try exact MEM1;
+      try exact PROMISE_SRC; try exact PROMISE; eauto.
+    { apply WF1_SRC. }
+    { apply WF1_TGT. }
+    { econs. apply TViewFacts.write_released_mon; try refl; ss.
+      - apply LOCAL1.
+      - apply WF1_TGT. }
+    i. des. inv MSG. esplits.
+    - econs; eauto.
+      + econs. inv WRITABLE.
+        eapply TimeFacts.le_lt_lt; eauto.
+        inv LOCAL1. inv TVIEW. inv CUR. ss.
+      + ii. inv LOCAL1.
+        exploit sim_promises_get_src; eauto. i. des. subst. ss.
+    - eauto.
+    - inv LOCAL1. econs; ss; eauto.
+      eapply TViewFacts.write_tview_mon; try refl; ss. apply WF1_TGT.
+    - ss.
+    - ss.
+  Qed.
+
+  Definition fence_step := PFStep.fence_step.
+
+  Inductive lower_cap (caps: TimeMap.t): forall (mem1 mem2: Memory.t), Prop :=
+  | lower_cap_refl mem:
+      lower_cap caps mem mem
+  | lower_cap_lower
+      mem1 mem2
+      loc from to val released
+      from_cap
+      (GET: Memory.get loc to mem1 = Some (from, Message.full val released))
+      (LOWER: Memory.lower mem1 loc from_cap (caps loc) Message.half (Message.full val None) mem2):
+      lower_cap caps mem1 mem2
+  .
+  Hint Constructors lower_cap.
+
+  Program Instance lower_cap_Reflexive: forall caps, Reflexive (lower_cap caps).
+
+  Inductive pf_step (lang: Language.t) (caps: TimeMap.t): forall (e1 e2: Thread.t lang), Prop :=
+  | pf_step_intro
+      e e1 st2 lc2 sc2 mem2 mem3
+      (STEP: @Thread.step lang true e e1 (Thread.mk lang st2 lc2 sc2 mem2))
+      (LOWER: @lower_cap caps mem2 mem3):
+      pf_step caps e1 (Thread.mk lang st2 lc2 sc2 mem3)
+  .
+  Hint Constructors pf_step.
+
+  Lemma pf_step_future
+        lang
+        latests caps e_tgt
+        e1 e2
+        (SIM: @sim_thread lang latests caps e2 e_tgt)
+        (STEP: pf_step caps e1 e2)
+        (WF1: Local.wf e1.(Thread.local) e1.(Thread.memory))
+        (SC1: Memory.closed_timemap e1.(Thread.sc) e1.(Thread.memory))
+        (CLOSED1: Memory.closed e1.(Thread.memory)):
+    <<WF2: Local.wf e2.(Thread.local) e2.(Thread.memory)>> /\
+    <<SC2: Memory.closed_timemap e2.(Thread.sc) e2.(Thread.memory)>> /\
+    <<CLOSED2: Memory.closed e2.(Thread.memory)>> /\
+    <<TVIEW_FUTURE: TView.le e1.(Thread.local).(Local.tview) e2.(Thread.local).(Local.tview)>> /\
+    <<SC_FUTURE: TimeMap.le e1.(Thread.sc) e2.(Thread.sc)>> /\
+    <<MEM_FUTURE: Memory.future e1.(Thread.memory) e2.(Thread.memory)>>.
+  Proof.
+    destruct e1, e2, e_tgt. ss. inv STEP.
+    exploit Thread.step_future; eauto. s. i. des.
+    inv LOWER; try by (esplits; eauto).
+    assert (FUTURE: Memory.future mem2 memory0).
+    { econs; eauto. econs; eauto. econs. ss.
+      unfold TimeMap.bot. apply Time.bot_spec. }
+    splits; auto.
+    - inv WF2. econs; eauto.
+      + eapply TView.future_closed; eauto.
+      + ii. exploit PROMISES; eauto. i.
+        erewrite Memory.lower_o; eauto. condtac; ss.
+        des. subst.
+        inv SIM. inv MEMORY. ss. specialize (CAPP loc).
+        inv LOCAL. inv PROMISES0.
+        exploit SOUND0; eauto. i. des. congr.
+    - eapply Memory.future_closed_timemap; eauto.
+    - eapply Memory.future_closed; eauto.
+    - etrans; eauto.
   Qed.
 
   Lemma program_step
+        latests caps
         lc1_src sc1_src mem1_src
         e_tgt lc1_tgt sc1_tgt mem1_tgt lc2_tgt sc2_tgt mem2_tgt
         (LOCAL1: sim_local lc1_src lc1_tgt)
         (SC1: TimeMap.le sc1_src sc1_tgt)
-        (MEM1: sim_memory lc1_tgt.(Local.promises) mem1_src mem1_tgt)
+        (MEM1: sim_memory latests caps lc1_tgt.(Local.promises) mem1_src mem1_tgt)
         (WF1_SRC: Local.wf lc1_src mem1_src)
         (WF1_TGT: Local.wf lc1_tgt mem1_tgt)
         (SC1_SRC: Memory.closed_timemap sc1_src mem1_src)
@@ -587,11 +1035,12 @@ Module CapPFStep.
         (CLOSED1_TGT: Memory.closed mem1_tgt)
         (STEP_TGT: Local.program_step e_tgt lc1_tgt sc1_tgt mem1_tgt lc2_tgt sc2_tgt mem2_tgt)
         (CONS: promise_consistent lc2_tgt):
-    exists e_src lc2_src sc2_src mem2_src,
+    exists e_src lc2_src sc2_src mem2_src mem3_src,
       <<STEP_SRC: Local.program_step e_src lc1_src sc1_src mem1_src lc2_src sc2_src mem2_src>> /\
+      <<LOWER: lower_cap caps mem2_src mem3_src>> /\
       <<LOCAL2: sim_local lc2_src lc2_tgt>> /\
       <<SC2: TimeMap.le sc2_src sc2_tgt>> /\
-      <<MEM2: sim_memory lc2_tgt.(Local.promises) mem2_src mem2_tgt>> /\
+      <<MEM2: sim_memory latests caps lc2_tgt.(Local.promises) mem3_src mem2_tgt>> /\
       <<EVENT: ThreadEvent.get_program_event e_src = ThreadEvent.get_program_event e_tgt>>.
   Proof.
     inv STEP_TGT.
@@ -599,17 +1048,33 @@ Module CapPFStep.
     - exploit read_step; eauto. i. des.
       esplits; try exact LOCAL2; eauto.
       inv LOCAL. ss.
-    - exploit write_step; try exact LOCAL; eauto. i. des.
-      esplits; try exact LOCAL2; eauto.
+    - destruct (Time.eq_dec to (latests loc)).
+      + subst. exploit write_step_cap; try exact LOCAL; eauto. i. des.
+        esplits; try exact LOCAL2; try exact MEM2; eauto.
+        inv STEP_SRC. exploit Memory.write_get2; eauto.
+        { apply CLOSED1_SRC. }
+        { apply WF1_SRC. }
+        i. des. eauto.
+      + exploit write_step; try exact LOCAL; eauto. i. des.
+        esplits; try exact LOCAL2; eauto.
     - exploit read_step; eauto.
       { eapply write_step_promise_consistent; eauto. }
       i. des.
       exploit Local.read_step_future; try exact LOCAL0; eauto. i. des.
       exploit Local.read_step_future; try exact STEP_SRC; eauto. i. des.
-      exploit write_step; try exact LOCAL2; eauto.
-      { inv LOCAL0. ss. }
-      i. des.
-      esplits; try exact LOCAL4; eauto.
+      destruct (Time.eq_dec tsw (latests loc)).
+      + subst. exploit write_step_cap; try exact LOCAL2; eauto.
+        { inv LOCAL0. eauto. }
+        i. des.
+        esplits; try exact LOCAL4; try exact MEM2; eauto.
+        inv STEP_SRC0. exploit Memory.write_get2; eauto.
+        { apply CLOSED1_SRC. }
+        { apply WF0. }
+        i. des. eauto.
+      + exploit write_step; try exact LOCAL2; eauto.
+        { inv LOCAL0. eauto. }
+        i. des.
+        esplits; try exact LOCAL4; eauto.
     - exploit fence_step; eauto. i. des.
       esplits; try exact LOCAL2; eauto.
       inv LOCAL. ss.
@@ -619,9 +1084,9 @@ Module CapPFStep.
   Qed.
 
   Lemma thread_promise_step
-        lang e1_src
+        lang latests caps e1_src
         pf e_tgt e1_tgt e2_tgt
-        (SIM1: @sim_thread lang e1_src e1_tgt)
+        (SIM1: @sim_thread lang latests caps e1_src e1_tgt)
         (WF1_SRC: Local.wf e1_src.(Thread.local) e1_src.(Thread.memory))
         (WF1_TGT: Local.wf e1_tgt.(Thread.local) e1_tgt.(Thread.memory))
         (SC1_SRC: Memory.closed_timemap e1_src.(Thread.sc) e1_src.(Thread.memory))
@@ -631,7 +1096,7 @@ Module CapPFStep.
         (STEP_TGT: Thread.promise_step pf e_tgt e1_tgt e2_tgt):
     exists e_src e2_src,
       <<STEP_SRC: Thread.promise_step true e_src e1_src e2_src>> /\
-      <<SIM2: sim_thread e2_src e2_tgt>>.
+      <<SIM2: sim_thread latests caps e2_src e2_tgt>>.
   Proof.
     destruct e1_src, e1_tgt, e2_tgt. ss.
     inv SIM1. inv STEP_TGT. ss. subst.
@@ -642,9 +1107,9 @@ Module CapPFStep.
   Qed.
 
   Lemma thread_program_step
-        lang e1_src
+        lang latests caps e1_src
         e_tgt e1_tgt e2_tgt
-        (SIM1: @sim_thread lang e1_src e1_tgt)
+        (SIM1: @sim_thread lang latests caps e1_src e1_tgt)
         (WF1_SRC: Local.wf e1_src.(Thread.local) e1_src.(Thread.memory))
         (WF1_TGT: Local.wf e1_tgt.(Thread.local) e1_tgt.(Thread.memory))
         (SC1_SRC: Memory.closed_timemap e1_src.(Thread.sc) e1_src.(Thread.memory))
@@ -653,22 +1118,25 @@ Module CapPFStep.
         (MEM1_TGT: Memory.closed e1_tgt.(Thread.memory))
         (STEP_TGT: Thread.program_step e_tgt e1_tgt e2_tgt)
         (CONS: promise_consistent e2_tgt.(Thread.local)):
-    exists e_src e2_src,
+    exists e_src e2_src mem2_src,
       <<STEP_SRC: Thread.program_step e_src e1_src e2_src>> /\
-      <<SIM2: sim_thread e2_src e2_tgt>>.
+      <<LOWER: lower_cap caps e2_src.(Thread.memory) mem2_src>> /\
+      <<SIM2: sim_thread latests caps
+                         (Thread.mk lang e2_src.(Thread.state) e2_src.(Thread.local) e2_src.(Thread.sc) mem2_src) e2_tgt>>.
   Proof.
     destruct e1_src, e1_tgt, e2_tgt. ss.
     inv SIM1. inv STEP_TGT. ss. subst.
     exploit program_step; try exact LOCAL; try exact MEMORY; eauto. i. des.
     esplits.
     - econs; try exact STEP_SRC. rewrite EVENT. eauto.
-    - econs; eauto.
+    - eapply LOWER.
+    - ss.
   Qed.
 
   Lemma thread_step
-        lang e1_src
+        lang latests caps e1_src
         pf e_tgt e1_tgt e2_tgt
-        (SIM1: @sim_thread lang e1_src e1_tgt)
+        (SIM1: @sim_thread lang latests caps e1_src e1_tgt)
         (WF1_SRC: Local.wf e1_src.(Thread.local) e1_src.(Thread.memory))
         (WF1_TGT: Local.wf e1_tgt.(Thread.local) e1_tgt.(Thread.memory))
         (SC1_SRC: Memory.closed_timemap e1_src.(Thread.sc) e1_src.(Thread.memory))
@@ -677,21 +1145,23 @@ Module CapPFStep.
         (MEM1_TGT: Memory.closed e1_tgt.(Thread.memory))
         (STEP_TGT: Thread.step pf e_tgt e1_tgt e2_tgt)
         (CONS: promise_consistent e2_tgt.(Thread.local)):
-    exists e_src e2_src,
-      <<STEP_SRC: Thread.step true e_src e1_src e2_src>> /\
-      <<SIM2: sim_thread e2_src e2_tgt>>.
+    exists e2_src,
+      <<STEP_SRC: pf_step caps e1_src e2_src>> /\
+      <<SIM2: sim_thread latests caps e2_src e2_tgt>>.
   Proof.
     inv STEP_TGT.
     - exploit thread_promise_step; eauto. i. des.
-      esplits; eauto. econs 1; eauto.
+      esplits; eauto.
+      destruct e2_src. econs; eauto. econs; eauto.
     - exploit thread_program_step; eauto. i. des.
-      esplits; eauto. econs 2; eauto.
+      esplits; eauto.
+      destruct e2_src. econs; eauto. econs 2; eauto.
   Qed.
 
   Lemma thread_rtc_all_step
-        lang e1_src
+        lang latests caps e1_src
         e1_tgt e2_tgt
-        (SIM1: @sim_thread lang e1_src e1_tgt)
+        (SIM1: @sim_thread lang latests caps e1_src e1_tgt)
         (WF1_SRC: Local.wf e1_src.(Thread.local) e1_src.(Thread.memory))
         (WF1_TGT: Local.wf e1_tgt.(Thread.local) e1_tgt.(Thread.memory))
         (SC1_SRC: Memory.closed_timemap e1_src.(Thread.sc) e1_src.(Thread.memory))
@@ -701,8 +1171,8 @@ Module CapPFStep.
         (STEPS_TGT: rtc (@Thread.all_step lang) e1_tgt e2_tgt)
         (CONS: promise_consistent e2_tgt.(Thread.local)):
     exists e2_src,
-      <<STEPS_SRC: rtc (union (@Thread.step lang true)) e1_src e2_src>> /\
-      <<SIM2: sim_thread e2_src e2_tgt>>.
+      <<STEPS_SRC: rtc (@pf_step lang caps) e1_src e2_src>> /\
+      <<SIM2: sim_thread latests caps e2_src e2_tgt>>.
   Proof.
     revert e1_src SIM1 WF1_SRC SC1_SRC MEM1_SRC.
     induction STEPS_TGT; eauto; i.
@@ -711,16 +1181,16 @@ Module CapPFStep.
     exploit thread_step; try exact STEP; eauto.
     { eapply rtc_all_step_promise_consistent; eauto. }
     i. des.
-    exploit Thread.step_future; try exact STEP_SRC; eauto. i. des.
+    exploit pf_step_future; try exact STEP_SRC; eauto. i. des.
     exploit IHSTEPS_TGT; try exact SIM2; eauto. i. des.
     esplits; try exact SIM0.
     econs 2; eauto.
   Qed.
 
   Lemma thread_rtc_tau_step
-        lang e1_src
+        lang latests caps e1_src
         e1_tgt e2_tgt
-        (SIM1: @sim_thread lang e1_src e1_tgt)
+        (SIM1: @sim_thread lang latests caps e1_src e1_tgt)
         (WF1_SRC: Local.wf e1_src.(Thread.local) e1_src.(Thread.memory))
         (WF1_TGT: Local.wf e1_tgt.(Thread.local) e1_tgt.(Thread.memory))
         (SC1_SRC: Memory.closed_timemap e1_src.(Thread.sc) e1_src.(Thread.memory))
@@ -730,8 +1200,8 @@ Module CapPFStep.
         (STEPS_TGT: rtc (@Thread.tau_step lang) e1_tgt e2_tgt)
         (CONS: promise_consistent e2_tgt.(Thread.local)):
     exists e2_src,
-      <<STEPS_SRC: rtc (union (@Thread.step lang true)) e1_src e2_src>> /\
-      <<SIM2: sim_thread e2_src e2_tgt>>.
+      <<STEPS_SRC: rtc (@pf_step lang caps) e1_src e2_src>> /\
+      <<SIM2: sim_thread latests caps e2_src e2_tgt>>.
   Proof.
     eapply thread_rtc_all_step; eauto.
     eapply rtc_implies; [|eauto].
